about to relax some abstractions

concurrency/Machine_ax.v
@@ -3,6 +3,10 @@ Require Import concurrency.Asm_core. (* for AxiomaticCoreSem.
                             stop importing Asm_core *)
 Require Import compcert.common.Values.
 Require Import compcert.common.AST.
+Require Import compcert.common.Memdata.
+Require Import Coq.ZArith.BinInt.
+Require Import compcert.lib.Integers.
+Import Int.
 Import List.
 Import List.ListNotations.
 Import AxCoreSem.
@@ -11,12 +15,27 @@ Import AxCoreSem.
 (** Thread identifiers -- assume natural numbers *)
 Notation tid := nat. 
 
+(** Labels should satisfy this interface *)
+Class Labels :=
+  { E       :> Type;
+    isRead  : E -> bool;
+    isWrite : E -> bool;
+    Spawn   : tid -> E;
+    loc     : E -> option (block * Z * Z);
+    mval    : E -> option (list memval)
+  }.
+
 (** Class of threadwise semantics *)
-Class Semantics (E: Type) :=
+Class Semantics `{lbl:Labels} :=
  {
    G: Type; (** Type of global environment *)
    C: Type; (** Type of state/core *)
-   Sem: @AxiomaticCoreSemantics G C E (** Threadwise semantics *)
+   Sem: @AxiomaticCoreSemantics G C E; (** Threadwise semantics *)
+   NoSpawn_threadstep:
+     forall genv c c' evl,
+       corestep Sem genv c c' evl ->
+       ~ exists j, In (Spawn j) evl;
+   NoSpawn_atexternal
  }.
 
 Class ThreadPool (C: Type) :=
@@ -32,66 +51,68 @@ Class ThreadPool (C: Type) :=
         getThread i (updThread i c tp) = Some c
   }.
 
-Notation "tp # i " := (getThread i tp) (at level 1) : Ax_scope.
-Notation "tp <- i , c" := (updThread i c tp) (at level 1): Ax_scope.
-Notation tstep := (corestep Sem).
+Notation "tp # i " := (getThread i tp) (at level 1) : tp_scope.
+Notation "tp <- i , c" := (updThread i c tp) (at level 1): tp_scope.
+Notation threadStep := (corestep Sem).
+
+(** Symbol for thread spawn external *)
+Notation CREATE_SIG := (mksignature (AST.Tint::AST.Tint::nil) None cc_default).
+Notation CREATE := (EF_external "spawn" CREATE_SIG).
 
 (** Definition of a generic axiomatic concurrency machine *)
 Module AxSem.
 Section AxSem.
 
   Context
-    {E : Type}
-    {sem : Semantics E}
+    {Lab : Labels}
+    {sem : Semantics}
     {threadpool : ThreadPool C}.
   
-  (* Instance FunPool : ThreadPool. *)
-  (* Proof. *)
-  (*   eapply Build_ThreadPool with *)
-  (*   (t := nat -> option C) *)
-  (*     (getThread := fun i tp => tp i) *)
-  (*     (updThread := fun i c tp => *)
-  (*                     fun j => if (PeanoNat.Nat.eq_dec i j) *)
-  (*                           then Some c else tp j). *)
-  (*   - intros. *)
-  (*     unfold getThread, updThread. *)
-  (*     destruct eq_dec.EqDec_nat; subst; *)
-  (*       [exfalso|]; now auto. *)
-  (*   - intros. *)
-  (*     unfold getThread, updThread. *)
-  (*     destruct (PeanoNat.Nat.eq_dec i i); now tauto. *)
-  (* Defined. *)
+  Class SyncSteps :=
+    {
+      (** External (sync) steps*)
+      syncStep: G -> C ->  C -> list E -> Prop;
+      NoSpawn_sync:
+        forall genv c c' evl,
+          corestep Sem genv c c' evl ->
+          ~ exists j, In (Spawn j) evl
+    }.
 
-  (** Parameterized over external (concurrent) steps*)
-  Variable cstep: G -> t -> tid -> list E -> t -> Prop.
 
+  Context {ssteps : SyncSteps}.
+
+  Open Scope tp_scope.
   Inductive step (genv:G) (tp : t) (i: tid): list E -> t -> Prop :=
-  | InternalStep:
+  | ThreadStep:
       forall c c' evl
         (Hget: getThread i tp = Some c)
-        (Hstep: tstep genv c c' evl),
+        (Hstep: threadStep genv c c' evl),
         step genv tp i evl (updThread i c' tp)
-  | ExternalStep:
-      forall  evl tp'
-         (Hcstep: cstep genv tp i evl tp'),
-        step genv tp i evl tp'.
+  | SyncStep:
+      forall  c c' evl
+        (Hget: getThread i tp = Some c)
+        (Hstep: syncStep genv c c' evl),
+        step genv tp i evl (updThread i c' tp)
+  | StepSpawn:
+      forall c c' c'' b ofs arg evargs evinit j
+        (Hcode: tp # i = Some c)
+        (Hat_external: at_external Sem genv c CREATE
+                                   ((Vptr b ofs) :: arg :: nil) evargs)
+        (Hafter_external: after_external Sem genv None c = Some c')
+        (Hinitial: initial_core Sem j genv (Vptr b ofs) [arg] c'' evinit)
+        (Hfresh: tp # j = None),
+        step genv tp i (evargs ++ [Spawn j]) ((tp <- i,c') <- j,c'').
 
 End AxSem.
 End AxSem.
 
-Require Import compcert.lib.Integers.
-Import Int.
 
 (** Definition of an axiomatic concurrency machine consisting of lock operations *)
 Module AxLockMachine.
-Section AxLockMachine.
 
-  (** Externals symbols and signatures. *)
+  (** Symbols and signatures for externals of the locks machine. *)
   Notation EXIT :=
     (EF_external "EXIT" (mksignature (AST.Tint::nil) None)).
-
-  Notation CREATE_SIG := (mksignature (AST.Tint::AST.Tint::nil) None cc_default).
-  Notation CREATE := (EF_external "spawn" CREATE_SIG).
 
   Notation MKLOCK :=
     (EF_external "makelock" (mksignature (AST.Tint::nil) None cc_default)).
@@ -103,28 +124,27 @@ Section AxLockMachine.
   Notation UNLOCK_SIG := (mksignature (AST.Tint::nil) None cc_default).
   Notation UNLOCK := (EF_external "release" UNLOCK_SIG).
 
+  Section AxLockMachine.
+
   (** Assume some threadwise semantics*)
   Context 
-    {E : Type}
-    {sem : Semantics E}.
+    {lbl : Labels}
+    {sem : Semantics}.
 
-  (** Parameterize over the events generated for each step of the
-      Lock machine (e.g. x86 generates different events than Power) *)
+  (** Parameterize over the events generated for each synchronization step
+      of the Lock machine (e.g. x86 generates different events than Power) *)
   Class LockSem :=
     { lockE     : block -> int -> list E; (** Given the lock address *) 
       unlockE   : block -> int -> list E; 
       mklockE   : block -> int -> list E;
-      freelockE : block -> int -> list E;
-      spawnE    : block -> int -> val -> tid -> list E (** Given the address of the code to be executed
-                                                  an argument passed by parent thread and
-                                                  the tid of the new thread*)
+      freelockE : block -> int -> list E
      }.
   
   Context {threadpool: ThreadPool C}
           {lockSem: LockSem}.
 
-  Open Scope Ax_scope.
-  (** Concurrent steps of the lock machine *)
+  Open Scope tp_scope.
+  (** Sync steps of the lock machine *)
   Inductive cstep {genv:G} (tp : t) (i : tid): list E -> t -> Prop :=
   | StepAcq:
       forall c c' b ofs evargs
